src/ProbabilisticProgramming/Monad.dfy
@@ -15,6 +15,7 @@ module Monad {
 
   // Equation (2.38)
   function Tail(s: Random.Bitstream): (s': Random.Bitstream) {
+    TailIsBitstream(s);
     (n: nat) => s(n+1)
   }
 
@@ -129,6 +130,9 @@ module Monad {
       Join(Join(fff))(s);
     }
   }
+
+  lemma {:axiom} TailIsBitstream(s: Random.Bitstream)
+    ensures Random.IsBitstream((n: nat) => s(n+1))
 
   // Equation (2.68) && (2.77)
   lemma {:axiom} CoinHasProbOneHalf(b: bool)
